Some about language

DFA.v
@@ -1,4 +1,4 @@
-Require Import List Ensembles.
+Require Import List.
 
 Require Import Fin.
 
@@ -6,43 +6,82 @@ Require Import Fin.
 Inductive ter : Type :=
 | T : nat -> ter.
 
+Definition word := list ter.
+
+Definition language := word -> Prop.
 
 (** The type of deterministic finite automata. ***)
 Record dfa : Type := mkDfa {
   states_n: nat;
   start: t states_n;
-  final: Ensemble (t states_n);
+  final: list (t states_n);
   next: (t states_n) -> ter -> (t states_n);
 }.
 
-
-Definition word := list ter.
-
-Definition language := word -> Prop.
-
-
-Fixpoint accepts (d : dfa) (s: t (states_n d)) (w: word) : Prop :=
-  match w with
-     | nil => In (t (states_n d)) (final d) s
-     | h :: t => accepts d (next d s h) t 
+Fixpoint final_state (d : dfa) (s: t (states_n d)) (w: word) : t (states_n d) :=
+   match w with
+     | nil => s 
+     | h :: t => final_state d (next d s h) t 
   end.
+
+Definition accepts (d : dfa) (s: t (states_n d)) (w: word) : Prop :=
+  In (final_state d s w) (final d). 
+    
+
+(** The type of deterministic finite automata. ***)
+Record s_dfa: Type := s_mkDfa {
+  s_states_n: nat;
+  s_start: t s_states_n;
+  s_final: t s_states_n;
+  s_next: (t s_states_n) -> ter -> (t s_states_n);
+}.
+
+Fixpoint s_final_state (d : s_dfa) (s: t (s_states_n d)) (w: word) : t (s_states_n d) :=
+   match w with
+     | nil => s 
+     | h :: t => s_final_state d (s_next d s h) t 
+  end.
+
+Definition s_accepts (d : s_dfa) (s: t (s_states_n d)) (w: word) : Prop :=
+  (s_final_state d s w) = (s_final d).
 
 Definition dfa_language (d : dfa) := (accepts d (start d)).
 
+Definition s_dfa_language (d : s_dfa) := (s_accepts d (s_start d)).
+
+
+
+Fixpoint split_dfa_list (d : dfa) (f_list : list (t (states_n d)))
+   : list s_dfa :=
+  match f_list with
+     | nil => nil
+     | h :: t => s_mkDfa (states_n d) (start d) h (next d) :: split_dfa_list d t
+  end.
+
+Definition split_dfa (d: dfa) := split_dfa_list d (final d).
+  
 Definition language_union (l1 l2 : language) := fun w => (l1 w) \/ (l2 w).
 
 Definition language_intersection (l1 l2 : language) := fun w => (l1 w) /\ (l2 w).
 
 Definition language_eq (l1  l2 : language) := forall w : word, l1 w <-> l2 w. 
 
+Lemma mk_laguage_eq : forall (l1 l2 : language), (forall w : word, l1 w -> l2 w) -> (forall w : word, l2 w -> l1 w) -> language_eq l1 l2. 
+Proof.
+  intros l1 l2 H1 H2.
+  unfold language_eq.
+  intro w.
+  split.
+  apply (H1 w).
+  apply (H2 w).
+Qed.
+
 
 Theorem th1 : forall l1 l2 l3 : language, language_eq (language_intersection l1 (language_union l2 l3)) (language_union (language_intersection l1 l2) (language_intersection l1 l3)).
 Proof.
   intros.
-  unfold language_eq.    
-  intros.
-  split.
-  intro.
+  apply mk_laguage_eq.
+  intros w H.   
   unfold language_intersection in H.
   destruct H.
   unfold language_union in H0.
@@ -55,7 +94,7 @@ Proof.
   unfold language_intersection.
   intuition.
 
-  intros.
+  intros w H.
   unfold language_union in H.
   destruct H.
   unfold language_intersection in H.
@@ -89,10 +128,7 @@ Lemma distr : forall (a b c : Prop), (a /\ c) -> a /\ (b \/ c).
 Proof.
   intros.
   destruct H.
-  split.
-  exact H.
-  right.
-  exact H0.
+  auto.
 Qed.
   
 Theorem th2 : forall (l2 : language) (ls : list language),
@@ -107,8 +143,7 @@ Proof.
   intros H0.
   unfold language_intersection in H0.
   destruct H0.
-  simpl in H0.
-  elim H0.
+  auto.
   intros a tail.
   intro HR.
   intro LI.
@@ -181,3 +216,12 @@ Proof.
   unfold language_intersection in H.
   exact H.
 Qed.
+
+Theorem T21: forall d : dfa, language_eq (dfa_language d) (language_list_union (map (s_dfa_language) (split_dfa d))).
+Proof.
+  intros.
+  apply mk_laguage_eq.
+  intros w H1.
+  unfold dfa_language in H1.
+  unfold accepts in H1.
+  unfold split_dfa.
